spec/Utils.ec
@@ -1,0 +1,58 @@
+
+require import AllCore List Distr RealExp IntDiv.
+
+from Jasmin require import JModel.
+
+require import Array32.
+
+pragma Goals : printall.
+
+abbrev (<=) (a b : W64.t) = W64.to_uint a <= W64.to_uint b.
+
+module M = {
+    proc __memcmp (a:W8.t Array32.t, b:W8.t Array32.t) : W64.t = {
+        var r:W64.t;
+        var are_equal:W64.t;
+        var acc:W8.t;
+        var i:W64.t;
+        var t:W8.t;
+        var _of_:bool;
+        var _cf_:bool;
+        var _sf_:bool;
+        var zf:bool;
+        var  _0:bool;
+        var  _1:W8.t;
+
+        r <- (W64.of_int (- 1));
+        are_equal <- (W64.of_int 0);
+        acc <- (W8.of_int 0);
+        i <- (W64.of_int 0);
+
+        while ((i \ult (W64.of_int 32))) {
+          t <- a.[(W64.to_uint i)];
+          t <- (t `^` b.[(W64.to_uint i)]);
+          acc <- (acc `|` t);
+          i <- (i + (W64.of_int 1));
+        }
+
+        (_of_, _cf_, _sf_,  _0, zf,  _1) <- AND_8 acc acc;
+        r <- (zf ? are_equal : r);
+        return (r);
+  }
+}.
+
+op mkarray : 'a list -> 'a Array32.t. (* This is from Array theory ? *)
+
+op memcmp (a b : W8.t list) : bool = a = b.
+
+op int_of_bool (b : bool) : int = if b then 0 else -1.
+
+lemma memcmp_imp_fun (a b : W8.t list) :
+    hoare [M.__memcmp : arg = (mkarray a, mkarray b) ==> res = W64.of_int (int_of_bool (memcmp a b))].
+proof.
+proc.
+auto.
+while (W64.zero <= i <= W64.of_int 32).
+  - simplify. admit.
+  - progress. admit.
+qed.
